Fix relation between buffers and initial memory
Generalize buffer reads so that general integer indexes can be used,
despite negative integers making no sense in this context, to avoid
problems in conversion operators. Thus lifted, the specification
lemmas become provable.

Common/Values.v
@@ -363,10 +363,17 @@ Qed.
 Module Buffer.
   Definition t : Type := nat + list value.
 
-  Definition nth_error (buf : (nat + list value)) (i : nat) : option value :=
-    match buf with
-    | inl n => if i <? n then Some Undef else None
-    | inr vs => List.nth_error vs i
+  Definition nth_error (buf : (nat + list value)) (i : Z) : option value :=
+    let read (i : nat) : option value :=
+        match buf with
+        | inl n => if i <? n then Some Undef else None
+        | inr vs => List.nth_error vs i
+        end
+    in
+    match i with
+    | Zpos n => read (Pos.to_nat n)
+    | Z0 => read 0
+    | Zneg _ => None
     end.
 
   Definition well_formed_buffer (buf : (nat + list value)) : bool :=
