Common/Memory.v
@@ -793,7 +793,7 @@ Module ComponentMemoryExtra.
     load m b i = load (fst (reserve_blocks m n)) b i.
   Admitted.
 
-  (* TODO: Move above. *)
+  (* TODO: Move above. (Not needed any more?) *)
   Lemma load_prealloc_offset bufs b o v :
     load (prealloc bufs) b o = Some v ->
     (o >= 0)%Z.
@@ -802,7 +802,7 @@ Module ComponentMemoryExtra.
   Lemma reserve_blocks_prealloc bufs n mem bufs' b buf o :
     reserve_blocks (prealloc bufs) n = (mem, bufs') ->
     bufs b = Some buf ->
-    load mem b o = Buffer.nth_error buf (Z.to_nat o).
+    load mem b o = Buffer.nth_error buf o.
   Proof.
     intros Hmem Hbuf.
     destruct (load (prealloc bufs) b o) as [v |] eqn:Hload.
@@ -811,21 +811,23 @@ Module ComponentMemoryExtra.
       rewrite Hmem in Hload'.
       rewrite Hload' -Hload load_prealloc Hbuf /Buffer.nth_error.
       destruct buf as [m | vs] eqn:Hcase1.
-      + pose proof Z2Nat.id _ (Z.ge_le _ _ Hoffset) as Hid.
-        apply Zge_is_le_bool in Hoffset. rewrite Hoffset.
-        admit. (* Complete case analysis. *)
-      + apply Zge_is_le_bool in Hoffset. rewrite Hoffset. (* Refactor? *)
-        reflexivity.
+      + apply Zge_is_le_bool in Hoffset. rewrite Hoffset.
+        destruct o as [| o | o]. (* Perhaps do this case analysis at the top? *)
+        * admit. (* easy *)
+        * admit. (* easy *)
+        * admit. (* contradiction *)
+      + destruct o as [| o | o]; reflexivity.
     - assert (Hdomm : b \in domm (prealloc bufs)) by admit. (* Easy. *)
       pose proof load_after_reserve_blocks_none _ _ _ n Hdomm Hload as Hload'.
       rewrite Hmem in Hload'.
       rewrite Hload' -Hload load_prealloc Hbuf /Buffer.nth_error.
       destruct buf as [m | vs] eqn:Hcase1.
-      + admit.
-      + destruct (0 <=? o)%Z eqn:Hcase2.
+      + destruct o as [| o | o].
+        * admit. (* easy *)
+        * admit. (* easy *)
         * reflexivity.
-        * (* Need more precise spec for buffer reads. *)
-  Abort.
+      + destruct o as [| o | o]; reflexivity.
+  Admitted.
 End ComponentMemoryExtra.
 
 Module Memory.
